Attempt to show AddBH’ing on the denotational side

Launchbury/Adequacy.thy
@@ -7,7 +7,216 @@ lemma VariableNoBH:
   assumes "\<Gamma> : e \<Down>\<^bsub>x # L\<^esub> \<Delta> : z"
   shows "\<Gamma> : Var x \<Down>\<^bsub>L\<^esub> (x, z) # delete x \<Delta> : z"
 sorry
+
+
+definition demand :: "CEnv => exp => nat option" where
+  "demand \<rho> e = (if (\<N>\<lbrakk>e\<rbrakk>\<^bsub>\<rho>\<^esub>)\<cdot>C\<^sup>\<infinity> \<noteq> \<bottom> then Some (LEAST n. (\<N>\<lbrakk>e\<rbrakk>\<^bsub>\<rho>\<^esub>)\<cdot>C\<^bsup>n\<^esup> \<noteq> \<bottom>) else None)"
+
+lemma finite_resources_suffice:
+  assumes "(\<N>\<lbrakk>e\<rbrakk>\<^bsub>\<rho>\<^esub>)\<cdot>C\<^sup>\<infinity> \<noteq> \<bottom>"
+  obtains n where "(\<N>\<lbrakk>e\<rbrakk>\<^bsub>\<rho>\<^esub>)\<cdot>C\<^bsup>n\<^esup> \<noteq> \<bottom>"
+  sorry
+
+lemma more_resources_suffice:
+  assumes "(\<N>\<lbrakk>e\<rbrakk>\<^bsub>\<rho>\<^esub>)\<cdot>C\<^bsup>n\<^esup> \<noteq> \<bottom>" and "n \<le> m"
+  shows "(\<N>\<lbrakk>e\<rbrakk>\<^bsub>\<rho>\<^esub>)\<cdot>C\<^bsup>m\<^esup> \<noteq> \<bottom>"
+  sorry
+
+lemma infinite_resources_suffice:
+  assumes "(\<N>\<lbrakk>e\<rbrakk>\<^bsub>\<rho>\<^esub>)\<cdot>C\<^bsup>n\<^esup> \<noteq> \<bottom>"
+  shows "(\<N>\<lbrakk>e\<rbrakk>\<^bsub>\<rho>\<^esub>)\<cdot>C\<^sup>\<infinity> \<noteq> \<bottom>"
+  sorry
+
+lemma demand_suffices:
+  assumes "(\<N>\<lbrakk>e\<rbrakk>\<^bsub>\<rho>\<^esub>)\<cdot>C\<^sup>\<infinity> \<noteq> \<bottom>"
+  shows "(\<N>\<lbrakk>e\<rbrakk>\<^bsub>\<rho>\<^esub>)\<cdot>C\<^bsup>the (demand \<rho> e)\<^esup> \<noteq> \<bottom>"
+  apply (simp add: assms demand_def)
+  apply (rule finite_resources_suffice[OF assms])
+  apply (rule LeastI)
+  apply assumption
+  done
+
+lemma not_bot_demand:
+  "(\<N>\<lbrakk>e\<rbrakk>\<^bsub>\<rho>\<^esub>)\<cdot>C\<^bsup>n\<^esup> \<noteq> \<bottom> \<longleftrightarrow> demand \<rho> e \<noteq> None \<and> n \<ge> the (demand \<rho> e)"
+proof(intro iffI)
+  assume "(\<N>\<lbrakk>e\<rbrakk>\<^bsub>\<rho>\<^esub>)\<cdot>C\<^bsup>n\<^esup> \<noteq> \<bottom>"
+  thus "demand \<rho> e \<noteq> None \<and> n \<ge> the (demand \<rho> e)"
+    by (auto intro: Least_le simp add: demand_def dest: infinite_resources_suffice)
+next
+  assume *: "demand \<rho> e \<noteq> None \<and> n \<ge> the (demand \<rho> e)"
+  then have "(\<N>\<lbrakk>e\<rbrakk>\<^bsub>\<rho>\<^esub>)\<cdot>C\<^sup>\<infinity> \<noteq> \<bottom>"
+    by (auto intro: Least_le simp add: demand_def dest: infinite_resources_suffice)
+  hence "(\<N>\<lbrakk>e\<rbrakk>\<^bsub>\<rho>\<^esub>)\<cdot>C\<^bsup>the (demand \<rho> e)\<^esup> \<noteq> \<bottom>" by (rule demand_suffices)
+  moreover from * have "n \<ge> the (demand \<rho> e)"..
+  ultimately
+  show "(\<N>\<lbrakk>e\<rbrakk>\<^bsub>\<rho>\<^esub>)\<cdot>C\<^bsup>n\<^esup> \<noteq> \<bottom>" by (rule more_resources_suffice)
+qed
+
+lemma infinity_bot_demand:
+  "(\<N>\<lbrakk>e\<rbrakk>\<^bsub>\<rho>\<^esub>)\<cdot>C\<^sup>\<infinity> = \<bottom> \<longleftrightarrow> demand \<rho> e = None"
+  by (metis demand_suffices infinite_resources_suffice nat_le_linear not_bot_demand)
+
+lemma demand_suffices':
+  assumes "demand \<rho> e = Some n"
+  shows "(\<N>\<lbrakk>e\<rbrakk>\<^bsub>\<rho>\<^esub>)\<cdot>C\<^bsup>n\<^esup> \<noteq> \<bottom>"
+  by (metis assms not_bot_demand option.distinct(1) order_refl the.simps)
+
+lemma demand_not_0: "demand \<rho> e \<noteq> Some 0"
+proof
+  assume "demand \<rho> e = Some 0"
+  hence "(\<N>\<lbrakk>e\<rbrakk>\<^bsub>\<rho>\<^esub>)\<cdot>C\<^bsup>0\<^esup> \<noteq> \<bottom>" by (rule demand_suffices')
+  thus False by simp
+qed
+
+lemma demand_Suc_Least:
+  assumes "demand \<rho> e \<noteq> None"
+  shows "demand \<rho> e = Some (Suc (LEAST n. (\<N>\<lbrakk>e\<rbrakk>\<^bsub>\<rho>\<^esub>)\<cdot>C\<^bsup>Suc n\<^esup> \<noteq> \<bottom>))"
+proof-
+  from assms
+  have "demand \<rho> e = Some (LEAST n. (\<N>\<lbrakk>e\<rbrakk>\<^bsub>\<rho>\<^esub>)\<cdot>C\<^bsup>n\<^esup> \<noteq> \<bottom>)" by (auto simp add: demand_def)
+  also
+  then obtain n where "(\<N>\<lbrakk>e\<rbrakk>\<^bsub>\<rho>\<^esub>)\<cdot>C\<^bsup>n\<^esup> \<noteq> \<bottom>" by (metis  demand_suffices')
+  hence "(LEAST n. (\<N>\<lbrakk>e\<rbrakk>\<^bsub>\<rho>\<^esub>)\<cdot>C\<^bsup>n\<^esup> \<noteq> \<bottom>) = Suc (LEAST n. (\<N>\<lbrakk>e\<rbrakk>\<^bsub>\<rho>\<^esub>)\<cdot>C\<^bsup>Suc n\<^esup> \<noteq> \<bottom>)"
+    by (rule Least_Suc) auto
+  finally show ?thesis.
+qed
+
+
+lemma demand_Var:
+  assumes "distinctVars \<Gamma>"
+  assumes "(x,e) \<in> set \<Gamma>"
+  shows "demand (\<N>\<lbrace>\<Gamma>\<rbrace>) (Var x) = Option.map Suc (demand (\<N>\<lbrace>\<Gamma>\<rbrace>) e)"
+proof(cases "(\<N>\<lbrakk>e\<rbrakk>\<^bsub>\<N>\<lbrace>\<Gamma>\<rbrace>\<^esub>)\<cdot>C\<^sup>\<infinity> = \<bottom>")
+  case True
+  with assms
+  have "(\<N>\<lbrakk>Var x\<rbrakk>\<^bsub>\<N>\<lbrace>\<Gamma>\<rbrace>\<^esub>)\<cdot>C\<^sup>\<infinity> = \<bottom>"
+    by (simp add: distinctVars_map_of heapVars_from_set)
+  with True
+  show ?thesis unfolding infinity_bot_demand by simp
+next
+  case False
+  with assms
+  have *: "(\<N>\<lbrakk>Var x\<rbrakk>\<^bsub>\<N>\<lbrace>\<Gamma>\<rbrace>\<^esub>)\<cdot>C\<^sup>\<infinity> \<noteq> \<bottom>"
+    by (simp add: distinctVars_map_of heapVars_from_set)
+  hence "demand (\<N>\<lbrace>\<Gamma>\<rbrace>) (Var x) \<noteq> None" by (metis infinity_bot_demand)
+
+  have [simp]: "x \<in> heapVars \<Gamma>" by (metis assms(2) heapVars_from_set)
+  have [simp]: "map_of \<Gamma> x = Some e" by (metis assms distinctVars_map_of)
+
+  have "demand (\<N>\<lbrace>\<Gamma>\<rbrace>) (Var x) = Some (Suc (LEAST n. (\<N>\<lbrakk>Var x\<rbrakk>\<^bsub>\<N>\<lbrace>\<Gamma>\<rbrace>\<^esub>)\<cdot>C\<^bsup>Suc n\<^esup> \<noteq> \<bottom>))"
+    by (rule demand_Suc_Least[OF `demand (\<N>\<lbrace>\<Gamma>\<rbrace>) (Var x) \<noteq> None`])
+  also have "\<dots> = Some (Suc (LEAST n. (\<N>\<lbrakk>e\<rbrakk>\<^bsub>\<N>\<lbrace>\<Gamma>\<rbrace>\<^esub>)\<cdot>C\<^bsup>n\<^esup> \<noteq> \<bottom>))" by simp
+  also have "\<dots> = Option.map Suc (demand (\<N>\<lbrace>\<Gamma>\<rbrace>) e)"
+    using False by (simp add: demand_def)
+  finally
+  show ?thesis.
+qed
+
+lemma demand_Var_there:
+  assumes "demand \<rho> (Var x) \<noteq> None"
+  shows "x \<in> fdom \<rho>"
+proof-
+  from assms obtain n where *: "(\<N>\<lbrakk>Var x\<rbrakk>\<^bsub>\<rho>\<^esub>)\<cdot>C\<^bsup>n\<^esup> \<noteq> \<bottom>"
+    by (metis not_bot_demand order_refl)
+  hence "n \<noteq> 0" by (auto intro: ccontr)
+  from * not0_implies_Suc[OF this]
+   show ?thesis by (auto intro: ccontr)
+qed
+
+lemma demand_Lam:
+  assumes "atom x \<sharp> \<rho>"
+  shows "demand \<rho> (Lam [x]. e') = Some 1"
+proof-
+  from assms
+  have "(\<N>\<lbrakk>Lam [x]. e'\<rbrakk>\<^bsub>\<rho>\<^esub>)\<cdot>C\<^bsup>1\<^esup> \<noteq> \<bottom>" by simp
+  hence "demand \<rho> (Lam [x]. e') \<noteq> None" and "the (demand \<rho> (Lam [x]. e')) \<le> 1"
+    by (metis not_bot_demand)+
+  with demand_not_0[where \<rho> = \<rho> and e = "Lam [x]. e'"]
+  show ?thesis by auto
+qed
+
+lemma demand_App:
+  shows "demand \<rho> (App e x) = undefined"
+proof(cases "demand \<rho> (App e x) = None")
+  case False
+  hence "demand \<rho> (App e x) = Some (Suc (LEAST n. (\<N>\<lbrakk>App e x\<rbrakk>\<^bsub>\<rho>\<^esub>)\<cdot>C\<^bsup>Suc n\<^esup> \<noteq> \<bottom>))" by (rule demand_Suc_Least)
+  also have "\<dots> = Some (Suc (LEAST n. ((\<N>\<lbrakk>e\<rbrakk>\<^bsub>\<rho>\<^esub>)\<cdot>C\<^bsup>n\<^esup> \<down>CFn (\<rho> f!\<^sub>\<bottom> x))\<cdot>C\<^bsup>n\<^esup> \<noteq> \<bottom>))" by simp
+  oops
+
+
+lemma
+  assumes "n < the (demand \<rho> (Var x))"
+  assumes "demand \<rho> e = Some n"
+  shows higher_demand_ignore: "demand \<rho> e = demand (fmap_delete x \<rho>) e"
+using assms
+proof(induction n arbitrary: \<rho> e)
+  case 0
+  from `demand \<rho> e = Some 0`
+  have False by (metis demand_not_0)
+  thus ?case..
+next
+  case (Suc n)
+  note d = `distinctVars \<Gamma>`
+  have "n < the (demand \<Gamma> (Var x))" using Suc(3) by simp
+  note prems = d this
+
+  show ?case
+  proof(cases e rule:exp_assn.strong_exhaust(1)[where c= \<Gamma>, case_names Var App Let Lam])
+    case (Var v)
+    note d2 = distinctVars_delete[OF d]
+
+    from Suc(3,4)[unfolded Var]
+    have "v \<noteq> x" by auto
+
+    from Suc(4)[unfolded Var]
+    have [simp]: "v \<in> heapVars \<Gamma>" by (auto intro: demand_Var_there)
+    then obtain e' where e': "(v,e') \<in> set \<Gamma>" by (auto simp add: heapVars_def)
+    with `v \<noteq> x` have e'': "(v, e') \<in> set (delete x \<Gamma>)" by (metis d distinctVars_map_of map_of_SomeD map_of_delete)
+
+    from Suc.prems(3)
+    have "demand \<Gamma> e' = Some n"  unfolding Var demand_Var[OF d e'] by simp
+    hence "demand \<Gamma> e' = demand (delete x \<Gamma>) e'"
+      by (rule Suc.IH[OF prems])
+    thus ?thesis
+      unfolding Var demand_Var[OF d e']  demand_Var[OF d2 e'']
+      by simp
+  next
+    case (Lam v e')
+    hence "atom v \<sharp> \<Gamma>" by (simp add: fresh_star_def)
+    moreover
+    hence "atom v \<sharp> delete x \<Gamma>" by (rule fresh_delete)
+    ultimately
+    show ?thesis
+      unfolding Lam by (simp only: demand_Lam)
+  next
+    case (Let e' v)
+    show ?thesis
+    
+    
+    
   
+
+  
+
+lemma add_BH:
+  assumes "distinctVars \<Gamma>"
+  assumes "(x, e) \<in> set \<Gamma>"
+  assumes  "(\<N>\<lbrakk>e\<rbrakk>\<^bsub>\<N>\<lbrace>\<Gamma>\<rbrace>\<^esub>)\<cdot>C\<^bsup>n\<^esup> \<noteq> \<bottom>"
+  shows "(\<N>\<lbrakk>e\<rbrakk>\<^bsub>\<N>\<lbrace>delete x \<Gamma>\<rbrace>\<^esub>)\<cdot>C\<^bsup>n\<^esup> \<noteq> \<bottom>"
+proof-
+  from assms
+  have "(\<N>\<lbrakk>Var x\<rbrakk>\<^bsub>\<N>\<lbrace>\<Gamma>\<rbrace>\<^esub>)\<cdot>C\<^bsup>Suc n\<^esup> \<noteq> \<bottom>"
+    by (simp add: distinctVars_map_of heapVars_from_set)
+  hence "demand \<Gamma> (Var x) \<noteq> None"  unfolding not_bot_demand by auto
+
+  from `demand \<Gamma> (Var x) \<noteq> None` demand_Var[OF assms(1,2)]
+  have "the (demand \<Gamma> (Var x)) = Suc (the (demand \<Gamma> e))" by auto
+  hence "the (demand \<Gamma> e) < the (demand \<Gamma> (Var x))" by simp
+  hence "demand \<Gamma> e = demand (delete x \<Gamma>) e" sorry
+  with assms(3)
+  show ?thesis unfolding not_bot_demand by simp
+qed
+
 
 theorem adequacy:
   assumes "(\<N>\<lbrakk>e\<rbrakk>\<^bsub>\<N>\<lbrace>\<Gamma>\<rbrace>\<^esub>)\<cdot>C\<^bsup>n\<^esup> \<noteq> \<bottom>"
@@ -30,10 +239,11 @@ next
     moreover
     from Suc.prems[unfolded Var] `(x, ?e) \<in> set \<Gamma>` `x \<in> heapVars \<Gamma>`
     have "(\<N>\<lbrakk>?e\<rbrakk>\<^bsub>\<N>\<lbrace>\<Gamma>\<rbrace>\<^esub>)\<cdot>C\<^bsup>n\<^esup> \<noteq> \<bottom>" by auto
-    from Suc.IH[OF this Suc.prems(2)]
-    obtain \<Delta> v where " \<Gamma> : ?e \<Down>\<^bsub>x # S\<^esub> \<Delta> : v" by blast
+    hence "(\<N>\<lbrakk>?e\<rbrakk>\<^bsub>\<N>\<lbrace>delete x \<Gamma>\<rbrace>\<^esub>)\<cdot>C\<^bsup>n\<^esup> \<noteq> \<bottom>" by (rule add_BH)
+    from Suc.IH[OF this distinctVars_delete[OF Suc.prems(2)]]
+    obtain \<Delta> v where "delete x \<Gamma> : ?e \<Down>\<^bsub>x # S\<^esub> \<Delta> : v" by blast
     ultimately
-    have "\<Gamma> : (Var x) \<Down>\<^bsub>S\<^esub> (x,v) # delete x \<Delta> : v" by (rule VariableNoBH)
+    have "\<Gamma> : (Var x) \<Down>\<^bsub>S\<^esub> (x,v) #  \<Delta> : v" by (rule Variable)
     thus ?thesis using Var by auto
   next
   case (App e' x)
